IEL refactor

pxl-minimal-kernel-main/.Makefile.d
@@ -6,8 +6,8 @@ coq/S5_Kripke.vo coq/S5_Kripke.glob coq/S5_Kripke.v.beautified coq/S5_Kripke.req
 coq/S5_Kripke.vos coq/S5_Kripke.vok coq/S5_Kripke.required_vos: coq/S5_Kripke.v 
 coq/PXL_Decidability.vo coq/PXL_Decidability.glob coq/PXL_Decidability.v.beautified coq/PXL_Decidability.required_vo: coq/PXL_Decidability.v 
 coq/PXL_Decidability.vos coq/PXL_Decidability.vok coq/PXL_Decidability.required_vos: coq/PXL_Decidability.v 
-coq/PXL_Completeness_Truth_WF.vo coq/PXL_Completeness_Truth_WF.glob coq/PXL_Completeness_Truth_WF.v.beautified coq/PXL_Completeness_Truth_WF.required_vo: coq/PXL_Completeness_Truth_WF.v 
-coq/PXL_Completeness_Truth_WF.vos coq/PXL_Completeness_Truth_WF.vok coq/PXL_Completeness_Truth_WF.required_vos: coq/PXL_Completeness_Truth_WF.v 
+coq/PXL_Completeness_Truth_WF.vo coq/PXL_Completeness_Truth_WF.glob coq/PXL_Completeness_Truth_WF.v.beautified coq/PXL_Completeness_Truth_WF.required_vo: coq/PXL_Completeness_Truth_WF.v coq/PXLv3.vo coq/PXL_Deep_Soundness.vo
+coq/PXL_Completeness_Truth_WF.vos coq/PXL_Completeness_Truth_WF.vok coq/PXL_Completeness_Truth_WF.required_vos: coq/PXL_Completeness_Truth_WF.v coq/PXLv3.vos coq/PXL_Deep_Soundness.vos
 coq/PXL_Completeness_Interface.vo coq/PXL_Completeness_Interface.glob coq/PXL_Completeness_Interface.v.beautified coq/PXL_Completeness_Interface.required_vo: coq/PXL_Completeness_Interface.v coq/PXLv3.vo
 coq/PXL_Completeness_Interface.vos coq/PXL_Completeness_Interface.vok coq/PXL_Completeness_Interface.required_vos: coq/PXL_Completeness_Interface.v coq/PXLv3.vos
 coq/PXL_Completeness_Instance.vo coq/PXL_Completeness_Instance.glob coq/PXL_Completeness_Instance.v.beautified coq/PXL_Completeness_Instance.required_vo: coq/PXL_Completeness_Instance.v coq/PXLv3.vo coq/PXL_Decidability.vo coq/PXL_Completeness_Interface.vo
