tests/HexiPraxis/HexiPraxis_Smoke.v
@@ -1,4 +1,4 @@
-﻿From Coq Require Import Program Setoids.Setoid.
+From Coq Require Import Program Setoids.Setoid.
 
 (* Standalone definitions for compilation - using PXL canonical model types *)
 Parameter form : Type.
@@ -17,20 +17,20 @@ Class Euclidean : Prop := { euclidean_R : forall w u v, can_R w u -> can_R w v -
 Class Serial : Prop := { serial_R : forall w, exists v, can_R w v }.
 
 (* Theorems from ModalPraxis *)
-Parameter provable_K : forall φ ψ, Prov (Impl (Box (Impl φ ψ)) (Impl (Box φ) (Box ψ))).
-Parameter provable_necessitation : forall φ, (forall w, forces w φ) -> Prov (Box φ).
-Parameter provable_D : Serial -> forall φ, Prov (Impl (Box φ) (Dia φ)).
-Parameter provable_4 : Transitive -> forall φ, Prov (Impl (Box φ) (Box (Box φ))).
-Parameter provable_5 : Euclidean -> forall φ, Prov (Impl (Dia φ) (Box (Dia φ))).
+Parameter provable_K : forall f g, Prov (Impl (Box (Impl f g)) (Impl (Box f) (Box g))).
+Parameter provable_necessitation : forall f, (forall w, forces w f) -> Prov (Box f).
+Parameter provable_D : Serial -> forall f, Prov (Impl (Box f) (Dia f)).
+Parameter provable_4 : Transitive -> forall f, Prov (Impl (Box f) (Box (Box f))).
+Parameter provable_5 : Euclidean -> forall f, Prov (Impl (Dia f) (Box (Dia f))).
 
 Module HexiPraxis.
 
-  (* Agents as parameters - agency logic [i]φ and ⟨i⟩φ *)
+  (* Agents as parameters - agency logic [i]f and ?i?f *)
   Parameter agent : Type.  (* Agents i, j, ... *)
 
-  (* Agency modalities: [i]φ means agent i brings about φ *)
-  Definition Brings_About (i:agent) (φ:form) : form := Box φ.
-  Definition Can_Bring_About (i:agent) (φ:form) : form := Dia φ.
+  (* Agency modalities: [i]f means agent i brings about f *)
+  Definition Brings_About (i:agent) (f:form) : form := Box f.
+  Definition Can_Bring_About (i:agent) (f:form) : form := Dia f.
 
   (* Frame classes for agency systems *)
   Class K_Frame : Prop := {}.  (* Basic agency logic *)
@@ -40,34 +40,34 @@ Module HexiPraxis.
                                agency_eucl : forall w u v, can_R w u -> can_R w v -> can_R u v }.
 
   (* Basic agency axioms *)
-  Theorem K_agency : K_Frame -> forall i φ ψ, Prov (Impl (Brings_About i (Impl φ ψ)) (Impl (Brings_About i φ) (Brings_About i ψ))).
-  Proof. intros _ i φ ψ; unfold Brings_About; apply provable_K. Qed.
+  Theorem K_agency : K_Frame -> forall i f g, Prov (Impl (Brings_About i (Impl f g)) (Impl (Brings_About i f) (Brings_About i g))).
+  Proof. intros _ i f g; unfold Brings_About; apply provable_K. Qed.
 
-  Theorem Necessitation_agency : K_Frame -> forall i φ, (forall w, forces w φ) -> Prov (Brings_About i φ).
-  Proof. intros _ i φ H; unfold Brings_About; apply provable_necessitation; exact H. Qed.
+  Theorem Necessitation_agency : K_Frame -> forall i f, (forall w, forces w f) -> Prov (Brings_About i f).
+  Proof. intros _ i f H; unfold Brings_About; apply provable_necessitation; exact H. Qed.
 
-  (* Success axiom: [i]φ → φ (agency implies truth) *)
-  Theorem Success : KD_Frame -> forall i φ, Prov (Impl (Brings_About i φ) φ).
-  Proof. intros H i φ; unfold Brings_About; destruct H as [Hser]; eapply provable_D; eauto. Qed.
+  (* Success axiom: [i]f ? f (agency implies truth) *)
+  Theorem Success : KD_Frame -> forall i f, Prov (Impl (Brings_About i f) f).
+  Proof. intros H i f; unfold Brings_About; destruct H as [Hser]; eapply provable_D; eauto. Qed.
 
-  (* Determinism under KD45: [i]φ → [i][i]φ *)
-  Theorem Determinism : KD45_Frame -> forall i φ, Prov (Impl (Brings_About i φ) (Brings_About i (Brings_About i φ))).
-  Proof. intros H i φ; unfold Brings_About; destruct H as [Hs Ht He]; eapply provable_4; eauto. Qed.
+  (* Determinism under KD45: [i]f ? [i][i]f *)
+  Theorem Determinism : KD45_Frame -> forall i f, Prov (Impl (Brings_About i f) (Brings_About i (Brings_About i f))).
+  Proof. intros H i f; unfold Brings_About; destruct H as [Hs Ht He]; eapply provable_4; eauto. Qed.
 
-  (* No learning under KD45: ⟨i⟩φ → [i]⟨i⟩φ *)
-  Theorem No_Learning : KD45_Frame -> forall i φ, Prov (Impl (Can_Bring_About i φ) (Brings_About i (Can_Bring_About i φ))).
-  Proof. intros H i φ; unfold Brings_About, Can_Bring_About; destruct H as [Hs Ht He]; eapply provable_5; eauto. Qed.
+  (* No learning under KD45: ?i?f ? [i]?i?f *)
+  Theorem No_Learning : KD45_Frame -> forall i f, Prov (Impl (Can_Bring_About i f) (Brings_About i (Can_Bring_About i f))).
+  Proof. intros H i f; unfold Brings_About, Can_Bring_About; destruct H as [Hs Ht He]; eapply provable_5; eauto. Qed.
 
 End HexiPraxis.
 
 Module T.
   Import HexiPraxis.
-  Lemma k_ok : K_Frame -> forall i φ ψ, Prov (Impl (Brings_About i (Impl φ ψ)) (Impl (Brings_About i φ) (Brings_About i ψ))).
+  Lemma k_ok : K_Frame -> forall i f g, Prov (Impl (Brings_About i (Impl f g)) (Impl (Brings_About i f) (Brings_About i g))).
   Proof. apply K_agency. Qed.
-  Lemma success_ok : KD_Frame -> forall i φ, Prov (Impl (Brings_About i φ) φ).
+  Lemma success_ok : KD_Frame -> forall i f, Prov (Impl (Brings_About i f) f).
   Proof. apply Success. Qed.
-  Lemma det_ok : KD45_Frame -> forall i φ, Prov (Impl (Brings_About i φ) (Brings_About i (Brings_About i φ))).
+  Lemma det_ok : KD45_Frame -> forall i f, Prov (Impl (Brings_About i f) (Brings_About i (Brings_About i f))).
   Proof. apply Determinism. Qed.
-  Lemma nolearn_ok : KD45_Frame -> forall i φ, Prov (Impl (Can_Bring_About i φ) (Brings_About i (Can_Bring_About i φ))).
+  Lemma nolearn_ok : KD45_Frame -> forall i f, Prov (Impl (Can_Bring_About i f) (Brings_About i (Can_Bring_About i f))).
   Proof. apply No_Learning. Qed.
 End T.
