modules/IEL/infra/ModalPraxis/ForcesLemmas.v
@@ -2,18 +2,29 @@ From PXLs.IEL.Infra.TropoPraxis Require Import Tropo.
 From PXLs.IEL.Infra.ChronoPraxis Require Import Core.
 From PXLs.IEL.Infra.ModalPraxis.theorems Require Import NormalBase.
 
-Section ForcesCaps.
-  Context {W:Type} (R: W -> W -> Prop) (forces: W -> Prop -> Prop).
+Section ForcesBindings.
+  Context {W:Type} (R:W->W->Prop) (forces: W -> Prop -> Prop).
 
-  Hypothesis forces_mp :
-    forall w φ ψ, forces w (φ -> ψ) -> forces w φ -> forces w ψ.
-  Hypothesis forces_K :
-    forall w φ ψ, (* validity (□(φ->ψ) -> (□φ -> □ψ)) in your encoding *) True.
+  (* Bind to NormalBase parameters *)
+  Lemma forces_mp_pxl : forall w φ ψ, forces w (φ -> ψ) -> forces w φ -> forces w ψ.
+  Proof. intros w φ ψ H1 H2. apply (proj2 (forces_impl w φ ψ) H1 H2). Qed.
+
+  Lemma forces_K_pxl : forall w φ ψ, forces w (φ -> ψ) -> forces w φ -> forces w ψ.
+  Proof. apply forces_mp_pxl. Qed.  (* same as mp *)
 
   Global Instance CapForcesImpl_inst : Cap_ForcesImpl W R forces :=
-    {| forces_impl_mp := forces_mp |}.
+    {| forces_impl_mp := forces_mp_pxl |}.
 
   Global Instance CapForcesBox_inst : Cap_ForcesBox W R forces :=
-    {| forces_box_K := fun w φ ψ Hf Hφ => forces_mp w φ ψ Hf Hφ
-     ; forces_box_N := fun w φ _ => φ (* adjust to your validity encoding *) |}.
-End ForcesCaps.
+    {| forces_box_K := fun w φ ψ Hf Hφ => forces_K_pxl w φ ψ Hf Hφ
+     ; forces_box_N := fun w φ H => valid_necessitation φ w H |}.
+
+  Lemma forces_monotone_pxl :
+    forall w φ ψ, (forall v, forces v (φ -> ψ)) -> forces w φ -> forces w ψ.
+  Proof.
+    intros w φ ψ Hvalid Hφ. specialize (Hvalid w). eapply forces_mp_pxl; eauto.
+  Qed.
+
+  Global Instance CapForcesDia_inst : Cap_ForcesDia W R forces :=
+    {| forces_dia_monotone := forces_monotone_pxl |}.
+End ForcesBindings.
