modules/IEL/infra/TopoPraxis/Core.v
@@ -1,0 +1,18 @@
+From Coq Require Import FunctionalExtensionality.
+
+Module TopoPraxis.
+  Class Isometry (A B : Type) := {
+    iso_f : A -> B;
+    iso_g : B -> A;
+    iso_fg : forall x, iso_f (iso_g x) = x;
+    iso_gf : forall x, iso_g (iso_f x) = x
+  }.
+
+  Theorem BC_invariant {A B} (I : Isometry A B) (P : B -> Prop) :
+    (forall x, P x) <-> (forall x, P (iso_f I x)).
+  Proof.
+    split; intros H x.
+    - apply H.
+    - rewrite <- iso_fg; apply H.
+  Qed.
+End TopoPraxis.
