modules/IEL/infra/TropoPraxis/theorems/Conservativity.v
@@ -1,3 +1,3 @@
-﻿From Coq Require Import Program Setoids.Setoid.
+From Coq Require Import Program Setoids.Setoid.
 Set Implicit Arguments.
 (* TropoPraxis Conservativity  prove modal-free/propositional conservativity here. *)
