modules/IEL/theorems/Conservativity.v
@@ -1,4 +1,0 @@
-From Coq Require Import Program.
-From PXLs Require Import PXLv3.
-Set Implicit Arguments.
-(*  Conservativity  prove modal-free/propositional conservativity here. *)
