tests/TychePraxis/TychePraxis_Smoke.v
@@ -1,4 +1,4 @@
-﻿From Coq Require Import QArith Program.
+From Coq Require Import QArith Program.
 (* From PXLs Require Import PXLv3.
 Require Import modules.IEL.TychePraxis.modal.ProbSpec. *)
 Goal True. exact I. Qed.
